
\subsection{Homework 2}

\begin{problem}
  Let \(D\) be the region in \(\mathbb{R}^{2}\) enclosed by the ellipse
  \[
\frac{x^{2}}{a^{2}} + \frac{y^{2}}{b^{2}} = 1
\]
  Denote the ellipse by \(\partial D\) and consider the paremtrization of \(\partial {D}\) given by
  \[
c(t) = (a\cos(2t), b\sin(2t))
\]
\end{problem}

\begin{solution}
  The period of \(\gamma\) is \(\pi\)
\end{solution}

\begin{solution}
  Using the given parametrization \(c\), we can apply Green's Theorem to find the area of \(D\) given by
  \[
A(D) = \frac{1}{2}\int^{\pi}_{0} a\cos(2t)[b\sin(2t)]' - b\sin(2t)[a\cos(2t)]'\dif t = \frac{1}{2}\int^{\pi}_{0} 2ab\cos^{2}(2t) + 2ab\sin^{2}(2t) \dif t
\]
  \[
= \int^{\pi}_{0} ab \dif t = \pi ab
\]
\end{solution}

\begin{solution}
  Consider the parametrization of the ellipse given by \(c(t) = (a\cos(2t), b\sin(2t))\), we previously found the area of this curve is given by \(\pi ab\). Now, observe that the length \(l\) of \(c\) is given by
  \[
l = \int^{\pi}_{0}\norm{c'} = \int^{\pi}_{0}\sqrt{a^{2}\sin^{2}(2t)+b^{2}\cos^{2}(2t)}\dif t
\]
By the isoperemtric inequality, the length \(l\) satisfies \(l \geq \pi \sqrt{ab}\). Furthermore, the theorem states that equality holds if and only if \(c\) is a circle which happens only if \(a = b\).
\end{solution}

\begin{problem}
  Let \(S^{2}\) denote the unit sphere \(x^{2} + y^{2} + z^{2} = 1\) and define the parametrization \(\sigma \colon U\rightarrow \mathbb{R}^{3}\) by
  \[
\sigma(\theta, \phi) = (\cos \theta \cos \phi, \cos \theta \sin \phi, \sin \phi)
\]
  where
  \[
U = \{(\theta,\phi) \in \mathbb{R}^{2} | -\frac{\pi}{2} < \theta < \frac{\pi}{2}, 0 < \phi < 2\pi\} \text{and} C = \{(x,0,z) \in S^{2} | x \geq 0 \}
\]
\end{problem}

\begin{solution}
  Let \((\theta_{0}, \phi_{0}) \in U\). For the curve \(\gamma_{1}(\theta) = \sigma(\theta, \phi_{0})\), the curvature is given by
  \[
\kappa_{1} = \norm{\gamma_{1}(\theta)''} = \norm{\sigma(\theta, \phi_{0})''} = \sqrt{\cos^{2}\theta \cos^{2}\phi_{0} + \cos^{2}\theta \sin^{2}\phi_{0} + \sin^{2}\phi}
\]
  \[
= \sqrt{\cos^{2}(\theta_{0}) + \sin^{2}(\phi)} = 1
\]
  and the curvature of the curve \(\gamma_{2}(\theta) = \sigma(\theta_{0}, \phi)\) is given by
  \[
\kappa_{2} = \norm{\gamma_{2}(\theta)''} = \norm{\sigma(\theta_{0}, \phi)''} = \sqrt{-\cos^{2}\theta_{0}\cos^{2}\phi + -\cos^{2}\theta_{0} \sin^{2}} = \cos\theta_{0}
\]
\end{solution}
